fix: make list operations consistent in the order of arguments to beq
List / Array / Vector operations currently do not agree on the order when calling `beq`:

- `elem`, `contains`, `replace`, `lookup` (and indirectly `insert`) use the `a == ·` convention (the parameter to the operation is at the left, and the tested list element is at the right), despite documentation claiming the opposite

- `erase`, `count` and `[fin]idxOf[?]` use the `· == a` convention (the tested list element is on the left, and the parameter to the operation is at the right)

This inconsistency results in undesirable behavior when operations are mixed. Consider `isPerm`, which checks if two lists have the same elements excluding order. One might expect `isPerm` to never return true when the two lists don't even agree on size; unfortunately that does not happen in the general case, because the cons case

``` lean
 | a :: l₁, l₂ => l₂.contains a && l₁.isPerm (l₂.erase a)
```

mixes operations of both conventions, so it is possible for `.contains a` to claim a match while the subsequent `.erase a` fails to find it.

This patch changes the operations in the second group (erase, count, [fin]idxOf[?]) to align them with the first convention.
It was chosen purely to minimize the required changes; a downside of the `a == ·` convention is that it sometimes results in unnatural statements like `some a == list[i]`.
For this reason and to minimize breakage, I avoided flipping the arguments on lemmas involving `LawfulBEq`.

After this patch, `isPerm` only does tests of the form `l₁[i] == l₂[i]`, consistent with `List.beq`.

src/Init/Data/Array/Basic.lean
@@ -1119,7 +1119,7 @@ Examples:
 -/
 @[inline, expose]
 def count {α : Type u} [BEq α] (a : α) (as : Array α) : Nat :=
-  countP (· == a) as
+  countP (a == ·) as
 
 /--
 Applies a function to each element of the array, returning the resulting array of values.
@@ -1320,7 +1320,7 @@ def findIdx (p : α → Bool) (as : Array α) : Nat := (as.findIdx? p).getD as.s
 
 def idxOfAux [BEq α] (xs : Array α) (v : α) (i : Nat) : Option (Fin xs.size) :=
   if h : i < xs.size then
-    if xs[i] == v then some ⟨i, h⟩
+    if v == xs[i] then some ⟨i, h⟩
     else idxOfAux xs v (i+1)
   else none
 decreasing_by simp_wf; decreasing_trivial_pre_omega
@@ -1352,7 +1352,7 @@ Examples:
  * `#["carrot", "potato", "broccoli"].idxOf "tomato" = 3`
  * `#["carrot", "potato", "broccoli"].idxOf "anything else" = 3`
 -/
-def idxOf [BEq α] (a : α) : Array α → Nat := findIdx (· == a)
+def idxOf [BEq α] (a : α) : Array α → Nat := findIdx (a == ·)
 
 /--
 Returns the index of the first element equal to `a`, or `none` if no element is equal to `a`.
